TODO.md
@@ -2,3 +2,4 @@
 * When we matched against ``Eq`` in monomorphization, we found that some type arguments of other constants got unified with ``Prop``, which created a bunch of junk lemma. Find out whether something similar happened in Duper.
 * Implement native interpretation and native proof reconstruction
 * Improve portfolio mode script. Download E and zipperposition from the web.
+* Use `zipWithIndex` instead of the reinvented one.
